tests/lean/run/dsimp1.lean
@@ -1,0 +1,18 @@
+def Nat.isZero (x : Nat) : Bool :=
+  match x with
+  | 0 => true
+  | x+1 => false
+
+example (x : Nat) : (1 + id x.succ.pred).isZero = false := by
+  dsimp
+  trace_state
+  simp [Nat.succ_add]
+  dsimp [Nat.isZero]
+
+@[simp] theorem isZero_succ (x : Nat) : (x + 1).isZero = false :=
+  rfl
+
+theorem ex1 (x : Nat) : (id x.succ.succ.pred).isZero = false := by
+  dsimp
+
+#print ex1
